Try a new value (and env) relation in clos_callProof
This breaks many of the cases Magnus proved (but should not be too hard
to fix). The App and Fn cases have been reproved; the hope is that the
new relation makes the evaluate_app case possible, but it's not obvious
yet that it's good enough.

Also deleted some old commented out proof, and added in comments some
example programs that motivate the need for a more flexible value
relation than previously.

compiler/backend/proofs/clos_callProofScript.sml
@@ -111,6 +111,24 @@ val recclosure_rel_def = Define`
        set (code_locs (MAP SND fns1)) DIFF domain (FST new_g) ⊆ l ∧
        set (GENLIST (λi. 2*i+loc) (LENGTH fns1)) ⊆ l`;
 
+val env_rel_def = Define`
+  env_rel R env1 env2 a es ⇔
+    if LENGTH env1 = LENGTH env2 then LIST_REL R env1 env2 else
+    ∀x. EXISTS (λ(n,p). fv1 (n+a+x) p) es ⇒
+        x < LENGTH env1 ∧ x < LENGTH env2 ∧
+        R (EL x env1) (EL x env2)`;
+
+val env_rel_mono = Q.store_thm("env_rel_mono[mono]",
+  `(∀x y. MEM x env1 ∧ MEM y env2 ∧ R x y ⇒ R' x y) ⇒
+   env_rel R env1 env2 a es ⇒
+   env_rel R' env1 env2 a es`,
+  rw[env_rel_def,MEM_EL,PULL_EXISTS,LIST_REL_EL_EQN]);
+
+val env_rel_cong = Q.store_thm("env_rel_cong[defncong]",
+  `(∀x y. MEM x env1 ∧ MEM y env2 ⇒ (R x y ⇔ R' x y))
+   ⇒ env_rel R env1 env2 a es = env_rel R' env1 env2 a es`,
+  rw[env_rel_def,MEM_EL,PULL_EXISTS,EQ_IMP_THM,LIST_REL_EL_EQN]);
+
 val v_rel_def = tDefine"v_rel"`
   (v_rel g l (Number i) v ⇔ v = Number i) ∧
   (v_rel g l (Word64 w) v ⇔ v = Word64 w) ∧
@@ -121,12 +139,14 @@ val v_rel_def = tDefine"v_rel"`
      ∃g0 loc vs2 env2 bod2.
        recclosure_rel g l g0 loc [(n,bod1)] [(n,bod2)] ∧
        v = Closure (SOME loc) vs2 env2 n bod2 ∧ loco = SOME loc ∧
-       LIST_REL (v_rel g l) vs1 vs2 ∧ LIST_REL (v_rel g l) env1 env2) ∧
+       LIST_REL (v_rel g l) vs1 vs2 ∧
+       env_rel (v_rel g l) env1 env2 0 [(n,bod2)]) ∧
   (v_rel g l (Recclosure loco vs1 env1 fns1 i) v ⇔
      ∃g0 loc vs2 env2 fns2.
        recclosure_rel g l g0 loc fns1 fns2 ∧
        v = Recclosure (SOME loc) vs2 env2 fns2 i ∧ loco = SOME loc ∧
-       LIST_REL (v_rel g l) vs1 vs2 ∧ LIST_REL (v_rel g l) env1 env2)`
+       LIST_REL (v_rel g l) vs1 vs2 ∧
+       env_rel (v_rel g l) env1 env2 (LENGTH fns2) fns2)`
   (WF_REL_TAC `measure (v_size o FST o SND o SND)` >> simp[v_size_def] >>
    rpt strip_tac >> imp_res_tac v_size_lemma >> simp[]);
 
@@ -760,7 +780,8 @@ val v_rel_subg = Q.store_thm("v_rel_subg",
     v_rel g l v1 v2 ∧ subg g g' ∧ l ⊆ l' ⇒
     v_rel g' l' v1 v2`,
   ho_match_mp_tac v_rel_ind
-  \\ rw[v_rel_def,recclosure_rel_def]
+  \\ rw[v_rel_def,env_rel_def,recclosure_rel_def]
+  \\ Cases_on`LENGTH env1 = LENGTH env2`
   \\ fsrw_tac[ETA_ss][PULL_FORALL]
   \\ rpt(
     qmatch_assum_abbrev_tac`LIST_REL (v_rel g l) l1 l2`
@@ -780,8 +801,9 @@ val v_rel_subg = Q.store_thm("v_rel_subg",
   \\ imp_res_tac calls_length
   \\ fs[quantHeuristicsTheory.LIST_LENGTH_2]
   \\ rveq \\ fs[]
-  \\ IF_CASES_TAC \\ fs[]
-  \\ metis_tac[subg_trans,SUBSET_DEF]);
+  \\ CASE_TAC \\ fs[] \\ rfs[]
+  \\ fs[EXISTS_MEM,EXISTS_PROD]
+  \\ metis_tac[subg_trans,SUBSET_DEF,MEM_EL]);
 
 val state_rel_subg = Q.store_thm("state_rel_subg",
   `subg g0 g ∧ state_rel g0 l0 s t ∧ l0 ⊆ l ∧ code_includes (SND g) t.code ⇒ state_rel g l s t`,
@@ -825,8 +847,13 @@ val dest_closure_v_rel_lookup = Q.store_thm("dest_closure_v_rel_lookup",
      calls (MAP SND xs) g01 = (ls,g1) ∧ n < LENGTH ls ∧
      subg (code_list (loc - 2*n) (ZIP (MAP FST xs,ls)) g1) g ∧
      ALOOKUP (SND g) (loc+1) = SOME (LENGTH env1,EL n ls) ∧
-     dest_closure (SOME loc) v2 env2 = SOME (Full_app (Call 0 (loc+1) (GENLIST Var (LENGTH env1))) (env2++l1') []) ∧
-     LIST_REL (v_rel g l) l1 l1'`,
+     dest_closure (SOME loc) v2 env2 = SOME (Full_app (Call 0 (loc+1) (GENLIST Var (LENGTH env1))) (env2++l1') [])
+     (* ∧ LIST_REL (v_rel g l) (TAKE (LENGTH env1) l1) l1' *)
+     (*
+     (l1' = if is_Recclosure v1 then GENLIST (Recclosure (SOME loc) [] foo xs) (LENGTH xs)
+            else [])
+            *)
+     `,
   rw[dest_closure_def]
   \\ every_case_tac \\ fs[v_rel_def,recclosure_rel_def]
   \\ rw[] \\ fs[check_loc_def] \\ rw[]
@@ -891,13 +918,19 @@ val dest_closure_v_rel_lookup = Q.store_thm("dest_closure_v_rel_lookup",
   \\ fs[calls_list_MAPi]
   \\ rfs[NOT_LESS_EQUAL]
   \\ fs[indexedListsTheory.EL_MAPi]
+  (*
   \\ conj_tac
   >- (
+  *)
+    \\
     fs[subg_def]
     \\ first_x_assum match_mp_tac
     \\ simp[ALOOKUP_code_list]
     \\ DEEP_INTRO_TAC some_intro
-    \\ simp[EL_ZIP,EL_MAP] )
+    \\ simp[EL_ZIP,EL_MAP]
+    (*
+    )
+    *)
     (*
     \\ simp[ALOOKUP_APPEND]
     \\ reverse BasicProvers.CASE_TAC
@@ -917,8 +950,8 @@ val dest_closure_v_rel_lookup = Q.store_thm("dest_closure_v_rel_lookup",
     \\ DEEP_INTRO_TAC some_intro
     \\ simp[EL_ZIP,EL_MAP] )
     *)
-  \\ simp[revtakerev,revdroprev]
-  \\ match_mp_tac EVERY2_APPEND_suff
+  \\ simp[revtakerev,revdroprev,TAKE_APPEND]
+  \\ TRY (match_mp_tac EVERY2_APPEND_suff)
   \\ fsrw_tac[ETA_ss][]
   \\ simp[LIST_REL_GENLIST]
   \\ simp[v_rel_def,recclosure_rel_def]
@@ -972,21 +1005,14 @@ val dest_closure_v_rel = Q.store_thm("dest_closure_v_rel",
    (case x1 of Partial_app c1 =>
      ∃c2. x2 = Partial_app c2 ∧ v_rel g l c1 c2
     | Full_app e1 args1 rest1 =>
-      ∃g0 fns1 loc i fns2 args2 rest2.
+      ∃g0 fns1 loc i fns2 args2 rest2 opt.
         x2 = Full_app (SND (EL i fns2)) args2 rest2 ∧
-        LIST_REL (v_rel g l) args1 args2 ∧
+        (* env_rel (v_rel g l) args1 args2 0 (MAP (λx. (0,x)) (MAP SND fns2)) ∧ *)
         LIST_REL (v_rel g l) rest1 rest2 ∧
         recclosure_rel g l g0 loc fns1 fns2 ∧
         i < LENGTH fns1 ∧
         EL i fns1 = (FST (EL i fns2), e1) ∧
-        FST (EL i fns2) ≤ LENGTH args2
-        (*
-        every_Fn_SOME [e1] ∧
-        every_Fn_vs_NONE [e1] ∧
-        set (code_locs [e1]) ⊆ EVEN ∧
-        ALL_DISTINCT (code_locs [e1]) *)(*∧
-        (∃e2 g0 g1.
-          calls [e1] g0 = ([e2],g1)*))`,
+        FST (EL i fns2) ≤ LENGTH args2)`,
   rw[dest_closure_def]
   \\ Cases_on`v1` \\ fs[v_rel_def]
   \\ rveq \\ fs[]
@@ -1005,14 +1031,17 @@ val dest_closure_v_rel = Q.store_thm("dest_closure_v_rel",
     \\ Cases_on`b` \\ fs[calls_list_def]
     \\ rpt conj_tac
     \\ TRY (match_mp_tac EVERY2_TAKE \\ fs[])
-    \\ match_mp_tac EVERY2_APPEND_suff
-    \\ fsrw_tac[ETA_ss][]
-    \\ match_mp_tac EVERY2_APPEND_suff \\ fs[]
-    \\ match_mp_tac EVERY2_DROP \\ fs[] )
+    \\ rveq
+    \\ fsrw_tac[ETA_ss][env_rel_def,fv1_thm,fv_GENLIST_Var]
+    \\ IF_CASES_TAC \\ fs[] \\ rveq \\ fs[]
+    \\ rpt (match_mp_tac EVERY2_APPEND_suff \\ fs[])
+    \\ TRY (match_mp_tac EVERY2_DROP \\ fs[] )
+    \\ rw[] \\ res_tac \\ fs[])
   >- (
     simp[v_rel_def]
     \\ asm_exists_tac
     \\ fsrw_tac[ETA_ss][]
+    \\ fs[recclosure_rel_def]
     \\ match_mp_tac EVERY2_APPEND_suff
     \\ fs[] )
   \\ fsrw_tac[ETA_ss][]
@@ -1033,8 +1062,14 @@ val dest_closure_v_rel = Q.store_thm("dest_closure_v_rel",
     \\ fsrw_tac[ETA_ss][]
     \\ match_mp_tac EVERY2_APPEND_suff \\ fs[] )
   \\ fs[revdroprev,revtakerev]
+  (*
+  \\ map_every qexists_tac[`g0`,`l1`,`loc`,`n`,`fns2`]
+  \\ simp[DROP_DROP_T,DROP_LENGTH_TOO_LONG,DROP_APPEND]
+  \\ REWRITE_TAC[CONJ_ASSOC]
+  *)
   \\ first_assum(part_match_exists_tac (el 4 o rev o strip_conj) o concl)
   \\ qexists_tac`n` \\ fs[]
+  (*
   \\ conj_tac
   >- (
     fs[v_rel_def,recclosure_rel_def]
@@ -1051,6 +1086,7 @@ val dest_closure_v_rel = Q.store_thm("dest_closure_v_rel",
     \\ ntac 2 strip_tac
     \\ qexists_tac`g0`
     \\ fsrw_tac[ETA_ss][] )
+  *)
   \\ match_mp_tac EVERY2_TAKE \\ fs[]);
 
 (*
@@ -1302,7 +1338,7 @@ val calls_correct = Q.store_thm("calls_correct",
     ALL_DISTINCT (code_locs xs) ∧
     DISJOINT (IMAGE SUC (set (code_locs xs))) (set (MAP FST (SND g0))) ∧
     l = set (code_locs xs) DIFF domain (FST g) ∧
-    LIST_REL (v_rel g1 l1) env1 env2 ∧
+    env_rel (v_rel g1 l1) env1 env2 0 (MAP (λx. (0,x)) xs) ∧
     state_rel g1 l1 s0 t0 ∧
     subg g g1 ∧ l ⊆ l1 ∧ DISJOINT l1 (domain (FST g1)) ∧ wfg g1 ∧
     code_includes (SND g) t0.code
@@ -1315,6 +1351,7 @@ val calls_correct = Q.store_thm("calls_correct",
     evaluate_app loco f args s0 = (res,s) ∧
     res ≠ Rerr (Rabort Rtype_error) ∧
     v_rel g l f f' ∧
+    (* check_args_if_call (domain (FST g)) f (LENGTH args) ∧ *)
     LIST_REL (v_rel g l) args args' ∧
     state_rel g l s0 t0 ∧
     wfg g ∧ DISJOINT l (domain (FST g))
@@ -1332,7 +1369,8 @@ val calls_correct = Q.store_thm("calls_correct",
     \\ rveq \\ fs[evaluate_def]
     \\ fs[code_locs_def]
     \\ metis_tac[state_rel_subg,SUBSET_REFL])
-  \\ conj_tac >-
+  \\ conj_tac >- cheat
+   (*
    (fs [evaluate_def,calls_def] \\ rw []
     \\ pairarg_tac \\ fs [] \\ rw []
     \\ Cases_on `evaluate ([x],env,s)` \\ fs []
@@ -1403,14 +1441,18 @@ val calls_correct = Q.store_thm("calls_correct",
     \\ Cases_on `q` \\ fs [] \\ rveq \\ fs []
     \\ imp_res_tac evaluate_IMP_LENGTH
     \\ fs [] \\ Cases_on `a` \\ fs [])
+    *)
   (* Var *)
   \\ conj_tac >- (
     fs [evaluate_def,calls_def] \\ rw []
+    \\ fs[env_rel_def,fv1_thm]
+    \\ every_case_tac
     \\ imp_res_tac LIST_REL_LENGTH \\ fs []
     \\ qexists_tac `0` \\ fs []
     \\ fs [LIST_REL_EL_EQN])
   (* If *)
-  \\ conj_tac >-
+  \\ conj_tac >- cheat
+   (*
    (fs [evaluate_def,calls_def] \\ rw []
     \\ pairarg_tac \\ fs [] \\ rw []
     \\ Cases_on `evaluate ([x1],env,s)` \\ fs []
@@ -1545,8 +1587,10 @@ val calls_correct = Q.store_thm("calls_correct",
       \\ drule evaluate_add_clock \\ fs []
       \\ disch_then (qspec_then `ck'` assume_tac)
       \\ qexists_tac `ck+ck'` \\ fs [AC ADD_COMM ADD_ASSOC]))
+    *)
   (* Let *)
-  \\ conj_tac >- (
+  \\ conj_tac >- cheat
+    (*
     fs [evaluate_def,calls_def] \\ rw []
     \\ pairarg_tac \\ fs [] \\ rw []
     \\ Cases_on `evaluate (xs,env,s)` \\ fs []
@@ -1612,9 +1656,10 @@ val calls_correct = Q.store_thm("calls_correct",
     \\ disch_then (qspec_then `ck'` assume_tac)
     \\ qexists_tac `ck+ck'` \\ fs [AC ADD_COMM ADD_ASSOC]
     \\ `[HD e2] = e2` by (imp_res_tac calls_sing \\ fs [])
-    \\ fs [])
+    \\ fs []*)
   (* Raise *)
-  \\ conj_tac >-
+  \\ conj_tac >- cheat
+   (*
    (fs [evaluate_def,calls_def] \\ rw []
     \\ pairarg_tac \\ fs [] \\ rw []
     \\ fs [evaluate_def]
@@ -1628,9 +1673,10 @@ val calls_correct = Q.store_thm("calls_correct",
     \\ qexists_tac `ck` \\ fs []
     \\ every_case_tac \\ fs [evalPropsTheory.result_rel_def,PULL_EXISTS]
     \\ rw [] \\ imp_res_tac evaluate_IMP_LENGTH
-    \\ Cases_on `a` \\ Cases_on `a'` \\ fs [])
+    \\ Cases_on `a` \\ Cases_on `a'` \\ fs [])*)
   (* Handle *)
-  \\ conj_tac >- (
+  \\ conj_tac >- cheat
+    (*
     fs [evaluate_def,calls_def] \\ rw []
     \\ pairarg_tac \\ fs [] \\ rw []
     \\ Cases_on `evaluate ([x1],env,s1)` \\ fs []
@@ -1697,9 +1743,10 @@ val calls_correct = Q.store_thm("calls_correct",
     \\ qpat_assum `_ = (Rerr _,t)` assume_tac
     \\ drule evaluate_add_clock \\ fs []
     \\ disch_then (qspec_then `ck'` assume_tac)
-    \\ qexists_tac `ck+ck'` \\ fs [AC ADD_COMM ADD_ASSOC])
+    \\ qexists_tac `ck+ck'` \\ fs [AC ADD_COMM ADD_ASSOC]*)
   (* Op *)
-  \\ conj_tac >-
+  \\ conj_tac >- cheat
+   (*
    (fs [evaluate_def,calls_def] \\ rw []
     \\ pairarg_tac \\ fs [] \\ rw []
     \\ fs [evaluate_def]
@@ -1716,7 +1763,7 @@ val calls_correct = Q.store_thm("calls_correct",
     \\ disch_then (qspec_then `op` mp_tac) \\ fs []
     THEN1 (every_case_tac \\ fs [])
     \\ rename1 `_ = Rval rr` \\ PairCases_on `rr`
-    \\ fs [] \\ rw [] \\ fs [])
+    \\ fs [] \\ rw [] \\ fs [])*)
   (* Fn *)
   \\ conj_tac >- (
     rw[evaluate_def]
@@ -1738,37 +1785,6 @@ val calls_correct = Q.store_thm("calls_correct",
     \\ fs[closed_Fn]
     \\ `subg g0 (insert_each x 1 g0)`
     by ( simp[subg_def,insert_each_subspt] \\ fs[wfg_def])
-    (*
-    \\ `subg g0 g`
-    by (
-      every_case_tac \\ fs[] \\ rw[]
-      \\ drule calls_subg
-      \\ qhdtm_x_assum`calls`kall_tac
-      \\ drule calls_subg
-      \\ (impl_tac >- (fs[ALL_DISTINCT_APPEND] \\ fs[wfg_def]))
-      \\ strip_tac
-      \\ (impl_tac >- (fs[ALL_DISTINCT_APPEND] \\ fs[wfg_def]))
-      \\ strip_tac \\ fs[]
-      \\ match_mp_tac subg_trans
-      \\ qpat_assum`subg g0 (insert_each _ _ _)`assume_tac
-      \\ asm_exists_tac \\ rw[]
-      \\ match_mp_tac subg_trans
-      \\ asm_exists_tac \\ simp[]
-      \\ fs[subg_def]
-      \\ fs[IS_SUFFIX_APPEND,GSYM ADD1]
-      \\ imp_res_tac calls_add_SUC_code_locs
-      \\ rfs[SUBSET_DEF]
-      \\ fs[ALL_DISTINCT_APPEND]
-      \\ metis_tac[numTheory.INV_SUC] )
-    *)
-    (*
-    \\ qpat_abbrev_tac`l = l0 ∪ _`
-    \\ `l0 ⊆ l` by simp[Abbr`l`]
-    \\ `state_rel g l s t0` by metis_tac[state_rel_subg]
-    *)
-    (*
-    \\ `subspt (FST g0) (FST g)` by fs[subg_def]
-    *)
     \\ CONV_TAC(RESORT_EXISTS_CONV(sort_vars["g0'"]))
     \\ qexists_tac`g0` \\ fs[]
     \\ fs[ALL_DISTINCT_APPEND]
@@ -1810,58 +1826,14 @@ val calls_correct = Q.store_thm("calls_correct",
     \\ fs[DISJOINT_SYM]
     \\ imp_res_tac calls_add_SUC_code_locs
     \\ fs[SUBSET_DEF,GSYM ADD1]
-    \\ TRY (Cases_on`new_g'` \\ fs[code_list_def,GSYM ADD1] \\ NO_TAC)
-    (*
-    \\ `subg g new_g'`
-    by (
-      match_mp_tac calls_subg_mono
-      \\ asm_exists_tac \\ fs[]
-      \\ metis_tac[] )
-    \\ fs[subg_def]
-    \\ imp_res_tac subspt_domain_SUBSET
-    \\ fs[SUBSET_DEF,domain_FST_insert_each]
-    *)
-    \\ rw[] \\ first_x_assum match_mp_tac
-    \\ rfs[wfg_def,PULL_EXISTS]
-    \\ metis_tac[]
-    (*
     \\ rpt conj_tac
+    \\ TRY (Cases_on`new_g'` \\ fs[code_list_def,GSYM ADD1] \\ NO_TAC)
     \\ TRY (
-      match_mp_tac (GEN_ALL state_rel_subg) \\ fs[]
-      \\ first_assum(part_match_exists_tac (el 2 o strip_conj) o concl)
-      \\ simp[] )
-    \\ TRY ( match_mp_tac subg_refl \\ fs[wfg_def] )
-    \\ TRY (
-      match_mp_tac (GEN_ALL (MP_CANON LIST_REL_mono))
-      \\ first_assum(part_match_exists_tac (last o strip_conj) o concl)
-      \\ metis_tac[v_rel_subg,SUBSET_DEF] )
-    \\ strip_tac
-    \\ `MEM (SUC x) (MAP FST (SND g))` by fs[wfg_def]
-    \\ metis_tac[numTheory.INV_SUC]
-    *)
-    (*
-    \\ TRY ( reverse conj_tac >- (
-      TRY (
-        reverse conj_tac >- (
-          spose_not_then strip_assume_tac
-          \\ imp_res_tac calls_domain
-          \\ imp_res_tac calls_add_SUC_code_locs
-          \\ `x ∉ set (code_locs [exp])` by fs[ALL_DISTINCT_APPEND]
-          \\ `x ∉ domain (FST g0)`
-          by (
-            fs[wfg_def]
-            \\ fs[SET_EQ_SUBSET,SUBSET_DEF,PULL_EXISTS]
-            \\ metis_tac[] )
-          \\ `MEM (SUC x) (MAP FST (SND g))`
-          by ( drule calls_wfg \\ fs[ALL_DISTINCT_APPEND,wfg_def] )
-          \\ fs[SUBSET_DEF]
-          \\ metis_tac[numTheory.INV_SUC] ))
-      \\ match_mp_tac subg_refl \\ fs[subg_def] ))
-    \\ match_mp_tac (GEN_ALL (MP_CANON LIST_REL_mono))
-    \\ first_assum(part_match_exists_tac (last o strip_conj) o concl)
-    \\ metis_tac[v_rel_subg,SUBSET_REFL]
-    *)
-    )
+      first_x_assum match_mp_tac
+      \\ rfs[wfg_def,PULL_EXISTS]
+      \\ metis_tac[] )
+    \\ fs[env_rel_def,fv1_thm,fv_GENLIST_Var]
+    \\ rw[] \\ imp_res_tac calls_fv_imp \\ fs[])
   (* Letrec *)
   \\ conj_tac >- cheat
   (* App *)
@@ -1883,10 +1855,6 @@ val calls_correct = Q.store_thm("calls_correct",
     \\ strip_tac
     \\ `g'' = g` by (every_case_tac \\ fs[])
     \\ rveq \\ fs[]
-    (*
-    \\ qpat_abbrev_tac`l = l0 ∪ _`
-    \\ `l0 ⊆ l` by simp[Abbr`l`]
-    *)
     \\ `wfg g'`
     by (
       match_mp_tac calls_wfg
@@ -1896,6 +1864,8 @@ val calls_correct = Q.store_thm("calls_correct",
     by (
       match_mp_tac calls_wfg
       \\ asm_exists_tac \\ fs[] )
+    \\ `env_rel (v_rel g1 l1) env env2 0 (MAP (λx. (0,x)) args)`
+    by ( fsrw_tac[ETA_ss][env_rel_def,fv1_thm,EXISTS_MAP,fv_exists] )
     \\ reverse BasicProvers.TOP_CASE_TAC \\ fs[]
     >- (
       strip_tac \\ rveq \\ rfs[]
@@ -1915,27 +1885,6 @@ val calls_correct = Q.store_thm("calls_correct",
         \\ imp_res_tac calls_add_SUC_code_locs
         \\ rfs[wfg_def,SUBSET_DEF,PULL_EXISTS]
         \\ metis_tac[])
-      (*
-      \\ qpat_abbrev_tac`l' = l0 ∪ _`
-      \\ `l' ⊆ l`
-      by (
-        rw[Abbr`l'`,Abbr`l`,SUBSET_DEF]
-        \\ spose_not_then strip_assume_tac
-        \\ imp_res_tac calls_add_SUC_code_locs
-        \\ `x ∉ set (code_locs [x1])` by (fs[ALL_DISTINCT_APPEND]\\ metis_tac[])
-        \\ `MEM (SUC x) (MAP FST (SND g))` by ( fs[wfg_def] )
-        \\ `¬MEM (SUC x) (MAP FST (SND g'))` by ( fs[wfg_def] )
-        \\ fs[SUBSET_DEF]
-        \\ metis_tac[numTheory.INV_SUC] )
-      \\ rfs[]
-      \\ disch_then(qspecl_then[`env2`,`t0`,`g'`]mp_tac)
-      \\ impl_tac
-      >- (
-        conj_tac
-        >- (
-          match_mp_tac (GEN_ALL (MP_CANON LIST_REL_mono))
-          \\ metis_tac[v_rel_subg]
-      *)
       \\ strip_tac
       \\ qexists_tac`ck`
       \\ imp_res_tac calls_length
@@ -1969,42 +1918,15 @@ val calls_correct = Q.store_thm("calls_correct",
       \\ rfs[wfg_def,SUBSET_DEF,PULL_EXISTS]
       \\ metis_tac[])
     \\ strip_tac \\ fs[]
-    (*
-    \\ qmatch_asmsub_abbrev_tac`v_rel g' l'`
-    \\ `l' ⊆ l`
-    by (
-      rw[Abbr`l'`,Abbr`l`,SUBSET_DEF]
-      \\ spose_not_then strip_assume_tac
-      \\ imp_res_tac calls_add_SUC_code_locs
-      \\ `x ∉ set (code_locs [x1])` by (fs[ALL_DISTINCT_APPEND]\\ metis_tac[])
-      \\ `MEM (SUC x) (MAP FST (SND g))` by ( fs[wfg_def] )
-      \\ `¬MEM (SUC x) (MAP FST (SND g'))` by ( fs[wfg_def])
-      \\ fs[SUBSET_DEF]
-      \\ metis_tac[numTheory.INV_SUC] )
-    *)
     \\ disch_then(qspecl_then[`env2`,`t`]mp_tac)
-    (* \\ `l0 ⊆ l'` by simp[Abbr`l'`] *)
     \\ disch_then(qspecl_then[`l1`,`g1`]mp_tac)
     \\ impl_tac
     >- (
       imp_res_tac evaluate_const \\ fs[]
-      (*
-      \\ match_mp_tac (GEN_ALL (MP_CANON LIST_REL_mono))
-      \\ metis_tac[v_rel_subg,subg_trans]
-      *)
-      \\ fs[SUBSET_DEF])
+      \\ fs[SUBSET_DEF]
+      \\ fs[env_rel_def,fv1_thm]
+      \\ IF_CASES_TAC \\ fs[])
     \\ strip_tac \\ rveq
-    (*
-    \\ qmatch_assum_abbrev_tac`state_rel g ll _ _`
-    \\ `ll ⊆ l`
-    by ( simp[Abbr`ll`,Abbr`l`,SUBSET_DEF] )
-    \\ `l' ⊆ ll ` by simp[Abbr`ll`]
-    \\ `subg g g`
-    by (
-      match_mp_tac subg_refl
-      \\ imp_res_tac calls_ALL_DISTINCT
-      \\ rfs[DISJOINT_SYM] )
-    *)
     \\ qpat_assum`_ = (ys,_)`mp_tac
     \\ qmatch_goalsub_abbrev_tac`COND b`
     \\ reverse IF_CASES_TAC \\ fs[]
@@ -2030,17 +1952,8 @@ val calls_correct = Q.store_thm("calls_correct",
       \\ imp_res_tac evaluate_length_imp
       \\ fs[quantHeuristicsTheory.LIST_LENGTH_2]
       \\ rveq \\ fs[]
-      (*
-      \\ drule (GEN_ALL evaluate_app_imp_clos_rel)
-      \\ disch_then drule
-      \\ impl_tac >- (CCONTR_TAC \\ fs[] \\ fs[])
-      \\ strip_tac
-      *)
       \\ first_x_assum drule
-      (*
-      \\ qmatch_assum_rename_tac `LIST_REL (v_rel g' l') ev1 ev2`
-      \\ `LIST_REL (v_rel g ll) ev1 ev2` by metis_tac[LIST_REL_mono,v_rel_subg]
-      *)
+      \\ qmatch_assum_rename_tac`LIST_REL (v_rel _ _) ev1 ev2`
       \\ disch_then drule
       \\ disch_then drule
       \\ impl_tac >- rw[]
@@ -2049,12 +1962,7 @@ val calls_correct = Q.store_thm("calls_correct",
       \\ disch_then(qspec_then`ck'+ck''`mp_tac) \\ simp[] \\ strip_tac
       \\ qpat_assum`evaluate([_],env2,_) = _`(mp_tac o MATCH_MP evaluate_add_clock)
       \\ disch_then(qspec_then`ck''`mp_tac) \\ simp[] \\ strip_tac
-      \\ qexists_tac`ck+ck'+ck''` \\ fs[]
-      (*
-      \\ conj_tac >- metis_tac[state_rel_subg,state_rel_def]
-      \\ Cases_on`res` \\ fs[] \\ TRY (Cases_on`e` \\ fs[])
-      \\ TRY (match_mp_tac (GEN_ALL (MP_CANON LIST_REL_mono)))
-      \\ metis_tac[v_rel_subg]*))
+      \\ qexists_tac`ck+ck'+ck''` \\ fs[])
     \\ qpat_assum`Abbrev(IS_SOME _ ∧ _)`mp_tac
     \\ simp[markerTheory.Abbrev_def,IS_SOME_EXISTS]
     \\ strip_tac \\ rveq \\ fs[]
@@ -2064,24 +1972,7 @@ val calls_correct = Q.store_thm("calls_correct",
       \\ imp_res_tac subspt_domain_SUBSET
       \\ fs[SUBSET_DEF] )
     \\ `x ∉ l1` by ( fs[IN_DISJOINT] \\ metis_tac[] )
-    (*
-    \\ `x ∉ ll`
-    by (
-      simp[Abbr`ll`]
-      \\ Cases_on`x ∈ domain (FST g')`
-      >- (fs[IN_DISJOINT] \\ metis_tac[])
-      \\ `wfg g'` by imp_res_tac calls_wfg
-      \\ `¬MEM (SUC x) (MAP FST (SND g'))` by fs[wfg_def]
-      \\ `MEM (SUC x) (MAP FST (SND g))` by fs[wfg_def]
-      \\ `MEM x (code_locs [x1])`
-      by (
-        imp_res_tac calls_add_SUC_code_locs
-        \\ fs[SUBSET_DEF]
-        \\ metis_tac[numTheory.INV_SUC] )
-      \\ `x ∉ l0` by (fs[IN_DISJOINT] \\ metis_tac[])
-      \\ simp[Abbr`l'`]
-      \\ fs[ALL_DISTINCT_APPEND] )
-    *)
+
     \\ IF_CASES_TAC \\ fs[] \\ strip_tac \\ rveq \\ fs[]
     \\ simp[evaluate_def]
     >- (
@@ -2093,10 +1984,6 @@ val calls_correct = Q.store_thm("calls_correct",
       \\ ntac 2 strip_tac \\ rveq
       \\ fs[quantHeuristicsTheory.LIST_LENGTH_2] \\ rveq
       \\ rfs[] \\ rveq
-      (*
-      \\ qmatch_assum_rename_tac `LIST_REL (v_rel g' l') ev1 ev2`
-      \\ `LIST_REL (v_rel g ll) ev1 ev2` by metis_tac[LIST_REL_mono,v_rel_subg]
-      *)
       \\ qmatch_assum_rename_tac`LIST_REL (v_rel g1 l1) ev1 ev2`
       \\ Cases_on`ev1 = []`
       \\ imp_res_tac evaluate_length_imp \\ rfs[]
@@ -2104,6 +1991,7 @@ val calls_correct = Q.store_thm("calls_correct",
       \\ qpat_assum`_ = (res,_)`mp_tac
       \\ BasicProvers.TOP_CASE_TAC \\ fs[]
       \\ strip_tac
+
       \\ drule (GEN_ALL dest_closure_v_rel_lookup)
       \\ disch_then drule
       \\ disch_then drule
@@ -2122,22 +2010,6 @@ val calls_correct = Q.store_thm("calls_correct",
           \\ rfs[wfg_def,GSYM ADD1] )
         \\ rpt(first_x_assum drule)
         \\ simp[] )
-      (*
-      by (
-        `ALL_DISTINCT (MAP FST (SND g1))` by fs[subg_def]
-        \\ `∃ls. SND g1 =  ls ++ SND g` by (metis_tac[subg_def,IS_SUFFIX_APPEND])
-        \\ pop_assum SUBST_ALL_TAC
-        \\ simp_tac(srw_ss())[ALOOKUP_APPEND]
-        \\ BasicProvers.CASE_TAC
-        \\ fs[ALL_DISTINCT_APPEND]
-        \\ imp_res_tac ALOOKUP_MEM
-        \\ `¬MEM (x+1) (MAP FST (SND g))`
-        by (
-          first_x_assum match_mp_tac
-          \\ simp[MEM_MAP,PULL_EXISTS]
-          \\ metis_tac[FST] )
-        \\ rfs[wfg_def,GSYM ADD1] )
-      *)
       \\ rfs[]
       \\ drule (GEN_ALL code_includes_ALOOKUP)
       \\ disch_then drule \\ strip_tac
@@ -2145,9 +2017,6 @@ val calls_correct = Q.store_thm("calls_correct",
       \\ first_x_assum drule
       \\ disch_then drule
       \\ qpat_assum`state_rel g1 l1 r t`assume_tac
-      (*
-      \\ `state_rel g ll r t` by ( metis_tac[state_rel_subg] )
-      *)
       \\ disch_then drule
       \\ impl_tac >- rw[]
       \\ strip_tac
@@ -2172,7 +2041,7 @@ val calls_correct = Q.store_thm("calls_correct",
       \\ IF_CASES_TAC
       >- (
         fs[] \\ strip_tac \\ rveq \\ fs[]
-        \\ `t'.clock = LENGTH ev2 - ck''` by decide_tac
+        \\ `t.clock = LENGTH ev2 - ck''` by decide_tac
         \\ fs[]
         \\ qexists_tac`ck` \\ simp[]
         \\ fs[dec_clock_def])
@@ -2217,16 +2086,12 @@ val calls_correct = Q.store_thm("calls_correct",
     \\ qpat_assum`LENGTH [_] = _`(assume_tac o SYM) \\ fs[]
     \\ fs[quantHeuristicsTheory.LIST_LENGTH_2] \\ rveq \\ fs[] \\ rveq
     \\ first_x_assum drule
-    (*
-    \\ qmatch_assum_rename_tac `LIST_REL (v_rel g' l') ev1 ev2`
-    \\ `LIST_REL (v_rel g ll) ev1 ev2` by metis_tac[LIST_REL_mono,v_rel_subg]
-    *)
-    \\ qmatch_assum_rename_tac`LIST_REL (v_rel _ _) ev1 ev2`
     \\ rpt(disch_then drule)
     \\ strip_tac
     \\ simp[find_code_def]
     \\ `t'.code = t0.code` by (imp_res_tac evaluate_const \\ fs[])
     \\ imp_res_tac evaluate_length_imp \\ fs[] \\ rw[]
+    \\ qmatch_assum_rename_tac`LIST_REL (v_rel g1 l1) ev1 ev2`
     \\ Cases_on`ev1 = []` \\ fs[]
     \\ fs[evaluate_app_rw]
     \\ qpat_assum`_ = (res,_)`mp_tac
@@ -2254,22 +2119,6 @@ val calls_correct = Q.store_thm("calls_correct",
         \\ rfs[wfg_def,GSYM ADD1] )
       \\ rpt(first_x_assum drule)
       \\ simp[] )
-    (*
-    by (
-      `ALL_DISTINCT (MAP FST (SND g1))` by fs[subg_def]
-      \\ `∃ls. SND g1 =  ls ++ SND g` by (metis_tac[subg_def,IS_SUFFIX_APPEND])
-      \\ pop_assum SUBST_ALL_TAC
-      \\ simp_tac(srw_ss())[ALOOKUP_APPEND]
-      \\ BasicProvers.CASE_TAC
-      \\ fs[ALL_DISTINCT_APPEND]
-      \\ imp_res_tac ALOOKUP_MEM
-      \\ `¬MEM (x+1) (MAP FST (SND g))`
-      by (
-        first_x_assum match_mp_tac
-        \\ simp[MEM_MAP,PULL_EXISTS]
-        \\ metis_tac[FST] )
-      \\ rfs[wfg_def,GSYM ADD1] )
-    *)
     \\ rfs[]
     \\ imp_res_tac code_includes_ALOOKUP \\ fs[]
     \\ IF_CASES_TAC \\ fs[]
@@ -2333,7 +2182,8 @@ val calls_correct = Q.store_thm("calls_correct",
     \\ TRY (Cases_on`e''` \\ fs[])
     \\ metis_tac[v_rel_subg])
   (* Tick *)
-  \\ conj_tac >-
+  \\ conj_tac >- cheat
+   (*
    (fs [evaluate_def,calls_def] \\ rw []
     \\ pairarg_tac \\ fs [] \\ rw []
     \\ `t0.clock = s.clock` by fs [state_rel_def]
@@ -2345,7 +2195,7 @@ val calls_correct = Q.store_thm("calls_correct",
     \\ rpt (disch_then drule)
     \\ disch_then (qspec_then `t0 with clock := t0.clock-1` mp_tac)
     \\ fs [] \\ impl_tac THEN1 fs [state_rel_def]
-    \\ strip_tac \\ asm_exists_tac \\ fs [])
+    \\ strip_tac \\ asm_exists_tac \\ fs []) *)
   (* Call *)
   \\ conj_tac >- (
     rw[evaluate_def,calls_def]
@@ -2362,12 +2212,13 @@ val calls_correct = Q.store_thm("calls_correct",
     \\ rw[evaluate_def]
     \\ first_x_assum drule
     \\ fs[code_locs_def]
+    \\ `env_rel (v_rel g1 l1) env env2 0 (MAP (λx. (0,x)) xs)`
+    by ( fsrw_tac[ETA_ss][env_rel_def,fv1_thm,EXISTS_MAP,fv_exists] )
     \\ disch_then drule \\ fs[]
     \\ rpt(disch_then drule) \\ rw[]
     \\ qexists_tac`ck`
     \\ rw[] )
   \\ conj_tac >- ( rw[evaluate_def] \\ qexists_tac`0` \\ rw[] )
-
   (* app cons *)
   \\ simp[evaluate_def]
   \\ rpt gen_tac \\ strip_tac
@@ -2404,6 +2255,7 @@ val calls_correct = Q.store_thm("calls_correct",
   \\ BasicProvers.TOP_CASE_TAC \\ fs[]
   \\ qmatch_assum_rename_tac`_ = (res',_)`
 
+  (*
   \\ Cases_on`res' = Rerr (Rabort Rtype_error)` \\ fs[]
   \\ reverse BasicProvers.TOP_CASE_TAC \\ fs[]
   >- (
@@ -2474,6 +2326,7 @@ val calls_correct = Q.store_thm("calls_correct",
       \\ qexists_tac`ck` \\ simp[] \\ rfs[] )
     \\ REWRITE_TAC[calls_list_MAPi]
     \\ simp[]
+
     \\ simp[evaluate_def,evaluate_GENLIST_Var]
     \\ simp[find_code_def]
     \\ simp[EVAL``(closSem$dec_clock _ _).code``]
@@ -2548,6 +2401,21 @@ val calls_correct = Q.store_thm("calls_correct",
   \\ fs[quantHeuristicsTheory.LIST_LENGTH_2]
   \\ strip_tac \\ rveq \\ fs[] \\ rfs[]
   \\ fs[PULL_EXISTS]
+  *)
   \\ cheat);
+
+(*
+val tm = ``closLang$Let [Op (Const 0) []; Op (Const 0) []]
+             (App NONE (Fn (SOME 1) NONE 1 (Fn (SOME 2) NONE 1 (Op (Const 1) []))) [Op (Const 2) []])``
+val res1 = EVAL``evaluate ([^tm],[],<|clock := 1|>)``
+val (ctm,ctab) = EVAL``clos_call$compile T ^tm`` |> concl |> rhs |> dest_pair
+val res2 = EVAL``evaluate ([^ctm],[],<|clock := 2; code := (alist_to_fmap ^ctab)|>)``
+
+val tm2 = ``closLang$Let [Op (Const 0) []; Op (Const 0) []]
+             (Fn (SOME 1) NONE 1 (App NONE (Fn (SOME 2) NONE 1 (Op (Const 1) [])) [Op (Const 2) []]))``
+val res3 = EVAL``evaluate ([^tm2],[],<|clock := 1|>)``
+val (ctm2,ctab2) = EVAL``clos_call$compile T ^tm2`` |> concl |> rhs |> dest_pair
+val res4 = EVAL``evaluate ([^ctm2],[],<|clock := 2; code := (alist_to_fmap ^ctab2)|>)``
+*)
 
 val _ = export_theory();
